Weidenbach_Book/IsaSAT_Setup_LLVM.thy
@@ -82,10 +82,28 @@ lemma restart_info_params[sepref_import_param]:
 type_synonym vmtf_node_assn = "(64 word \<times> 32 word \<times> 32 word)"    
 
 definition "vmtf_node1_rel \<equiv> { ((a,b,c),(VMTF_Node a b c)) | a b c. True}"
-definition "vmtf_node2_assn \<equiv> uint64_nat_assn *a snat_option_assn' TYPE(32) *a snat_option_assn' TYPE(32)"
+definition "vmtf_node2_assn \<equiv> uint64_nat_assn *a atom.option_assn *a atom.option_assn"
 
 definition "vmtf_node_assn \<equiv> hr_comp vmtf_node2_assn vmtf_node1_rel"
 lemmas [fcomp_norm_unfold] = vmtf_node_assn_def[symmetric]
+
+
+lemma vmtf_node_assn_pure[safe_constraint_rules]: \<open>CONSTRAINT is_pure vmtf_node_assn\<close>
+  unfolding vmtf_node_assn_def vmtf_node2_assn_def
+  by solve_constraint
+
+
+(*
+
+  TODO: Test whether this setup is safe in general? 
+    E.g., synthesize destructors when side-tac can prove is_pure.
+  
+lemmas [sepref_frame_free_rules] = mk_free_is_pure
+lemmas [simp] = vmtf_node_assn_pure[unfolded CONSTRAINT_def]
+*)
+
+lemmas [sepref_frame_free_rules] = mk_free_is_pure[OF vmtf_node_assn_pure[unfolded CONSTRAINT_def]]  
+
 
 lemma 
     vmtf_Node_refine1: "(\<lambda>a b c. (a,b,c), VMTF_Node) \<in> Id \<rightarrow> Id \<rightarrow> Id \<rightarrow> vmtf_node1_rel"
@@ -94,18 +112,18 @@ and vmtf_get_prev_refine1: "(\<lambda>(a,b,c). b, get_prev) \<in> vmtf_node1_rel
 and vmtf_get_next_refine1: "(\<lambda>(a,b,c). c, get_next) \<in> vmtf_node1_rel \<rightarrow> \<langle>Id\<rangle>option_rel"  
   by (auto simp: vmtf_node1_rel_def)
 
-sepref_definition VMTF_Node_impl is "uncurry2 (RETURN ooo (\<lambda>a b c. (a,b,c)))" :: "uint64_nat_assn\<^sup>k *\<^sub>a (snat_option_assn' TYPE(32))\<^sup>k *\<^sub>a (snat_option_assn' TYPE(32))\<^sup>k \<rightarrow>\<^sub>a vmtf_node2_assn"
+sepref_definition VMTF_Node_impl is "uncurry2 (RETURN ooo (\<lambda>a b c. (a,b,c)))" :: "uint64_nat_assn\<^sup>k *\<^sub>a (atom.option_assn)\<^sup>k *\<^sub>a (atom.option_assn)\<^sup>k \<rightarrow>\<^sub>a vmtf_node2_assn"
   unfolding vmtf_node2_assn_def by sepref
 
 sepref_definition VMTF_stamp_impl is "RETURN o (\<lambda>(a,b,c). a)" :: "vmtf_node2_assn\<^sup>k \<rightarrow>\<^sub>a uint64_nat_assn"
   unfolding vmtf_node2_assn_def 
   by sepref
 
-sepref_definition VMTF_get_prev_impl is "RETURN o (\<lambda>(a,b,c). b)" :: "vmtf_node2_assn\<^sup>k \<rightarrow>\<^sub>a snat_option_assn' TYPE(32)"
+sepref_definition VMTF_get_prev_impl is "RETURN o (\<lambda>(a,b,c). b)" :: "vmtf_node2_assn\<^sup>k \<rightarrow>\<^sub>a atom.option_assn"
   unfolding vmtf_node2_assn_def 
   by sepref
 
-sepref_definition VMTF_get_next_impl is "RETURN o (\<lambda>(a,b,c). c)" :: "vmtf_node2_assn\<^sup>k \<rightarrow>\<^sub>a snat_option_assn' TYPE(32)"
+sepref_definition VMTF_get_next_impl is "RETURN o (\<lambda>(a,b,c). c)" :: "vmtf_node2_assn\<^sup>k \<rightarrow>\<^sub>a atom.option_assn"
   unfolding vmtf_node2_assn_def 
   by sepref
 
@@ -127,8 +145,8 @@ type_synonym vmtf_remove_assn = \<open>vmtf_assn \<times> (32 word array_list64 
 
 
 abbreviation vmtf_assn :: "_ \<Rightarrow> vmtf_assn \<Rightarrow> assn" where
-  \<open>vmtf_assn \<equiv> (array_assn vmtf_node_assn *a uint64_nat_assn *a uint32_nat_assn *a uint32_nat_assn
-    *a snat_option_assn' TYPE(32))\<close>
+  \<open>vmtf_assn \<equiv> (array_assn vmtf_node_assn *a uint64_nat_assn *a atom_assn *a atom_assn
+    *a atom.option_assn)\<close>
 
 abbreviation atoms_hash_assn :: \<open>bool list \<Rightarrow> 1 word ptr \<Rightarrow> assn\<close> where
   \<open>atoms_hash_assn \<equiv> array_assn bool1_assn\<close>
@@ -274,7 +292,7 @@ sepref_definition access_lit_in_clauses_heur_fast_code
   supply [simp] = max_snat_def max_sint_def sint64_max_def
   unfolding isasat_bounded_assn_def access_lit_in_clauses_heur_alt_def
     access_lit_in_clauses_heur_pre_def
-  by sepref
+  by sepref (* slow *)
 
 declare access_lit_in_clauses_heur_fast_code.refine[sepref_fr_rules]
 
@@ -312,7 +330,7 @@ sepref_definition rewatch_heur_st_fast_code
   supply [[goals_limit=1]]
   unfolding rewatch_heur_st_def PR_CONST_def rewatch_heur_st_fast_pre_def
     isasat_bounded_assn_def rewatch_heur_st_fast_def
-  by sepref
+  by sepref (* slow *)
 
 declare rewatch_heur_st_fast_code.refine[sepref_fr_rules]
 
