Weidenbach_Book/IsaSAT_Trail_LLVM.thy
@@ -69,6 +69,7 @@ sepref_definition count_decided_pol_impl is "RETURN o count_decided_pol" :: "tra
 
 lemmas [sepref_fr_rules] = count_decided_pol_impl.refine
 
+
 sepref_definition get_level_atm_fast_code [llvm_code]
   is \<open>uncurry (RETURN oo get_level_atm_pol)\<close>
   :: \<open>[get_level_atm_pol_pre]\<^sub>a
@@ -78,7 +79,6 @@ sepref_definition get_level_atm_fast_code [llvm_code]
   supply [[eta_contract = false, show_abbrevs=false]]
   apply (rewrite at "nth _" eta_expand)
   apply (rewrite at "nth _ _" annot_index_of_atm)
-  supply [[goals_limit = 1]]
   by sepref
 
 declare get_level_atm_fast_code.refine[sepref_fr_rules]
@@ -152,9 +152,8 @@ sepref_definition tl_trail_tr_fast_code
         trail_pol_fast_assn\<^sup>d \<rightarrow> trail_pol_fast_assn\<close>
   supply if_splits[split] option.splits[split]
   unfolding tl_trailt_tr_def UNSET_def[symmetric] tl_trailt_tr_pre_def
-  unfolding trail_pol_fast_assn_def annot_index_atm_of
+  unfolding trail_pol_fast_assn_def
   apply (annot_unat_const "TYPE(32)")
-  (*apply (rewrite at \<open>_ - one_uint32_nat\<close> fast_minus_def[symmetric])*)
   supply [[goals_limit = 1]]
   by sepref
 
@@ -167,8 +166,8 @@ sepref_definition tl_trail_proped_tr_fast_code
         trail_pol_fast_assn\<^sup>d \<rightarrow> trail_pol_fast_assn\<close>
   supply if_splits[split] option.splits[split]
   unfolding tl_trail_propedt_tr_def UNSET_def[symmetric]
-    tl_trail_propedt_tr_pre_def annot_index_atm_of
-  unfolding ins_idx_upcast64[where i="atm_of _"] trail_pol_fast_assn_def
+    tl_trail_propedt_tr_pre_def
+  unfolding (*ins_idx_upcast64[where i="atm_of _"]*) trail_pol_fast_assn_def
   apply (annot_unat_const "TYPE(32)")
   supply [[goals_limit = 1]]
   by sepref
@@ -189,7 +188,7 @@ sepref_definition cons_trail_Decided_tr_fast_code
        unat_lit_assn\<^sup>k *\<^sub>a trail_pol_fast_assn\<^sup>d \<rightarrow> trail_pol_fast_assn\<close>
   unfolding cons_trail_Decided_tr_def cons_trail_Decided_tr_def trail_pol_fast_assn_def
     SET_TRUE_def[symmetric] SET_FALSE_def[symmetric] cons_trail_Decided_tr_pre_def
-  unfolding annot_index_atm_of
+  (*unfolding annot_index_atm_of*)
   apply (annot_unat_const "TYPE(32)")
   apply (rewrite at "_@[\<hole>]" in "(_,\<hole>)" annot_snat_unat_downcast[where 'l="32"])
   supply [[goals_limit = 1]]
@@ -216,7 +215,7 @@ sepref_definition get_propagation_reason_fast_code
   is \<open>uncurry get_propagation_reason_raw_pol\<close>
   :: \<open>trail_pol_fast_assn\<^sup>k *\<^sub>a unat_lit_assn\<^sup>k \<rightarrow>\<^sub>a sint64_nat_assn\<close>
   unfolding get_propagation_reason_raw_pol_def trail_pol_fast_assn_def
-    annot_index_atm_of
+    (*annot_index_atm_of*)
   by sepref
 
 declare get_propagation_reason_fast_code.refine[sepref_fr_rules]
@@ -265,7 +264,7 @@ sepref_definition tl_trail_tr_no_CS_fast_code
         trail_pol_fast_assn\<^sup>d \<rightarrow> trail_pol_fast_assn\<close>
   supply if_splits[split] option.splits[split]
   unfolding tl_trailt_tr_no_CS_def UNSET_def[symmetric] tl_trailt_tr_no_CS_pre_def
-  unfolding annot_index_atm_of trail_pol_fast_assn_def
+  unfolding (*annot_index_atm_of*) trail_pol_fast_assn_def
   apply (annot_unat_const "TYPE(32)")
   supply [[goals_limit = 1]]
   by sepref
